isabelle/Distinct_Elems/Algo_Transforms/Distinct_Elems_Algo_Transforms_Lazy.thy
@@ -8,8 +8,8 @@ imports
 
 begin
 
-definition lazy_step_1 :: "'a list \<Rightarrow> nat \<Rightarrow> 'a state \<Rightarrow> 'a state pmf"
-  where "lazy_step_1 xs i state = do {
+definition step_1_lazy :: "'a list \<Rightarrow> nat \<Rightarrow> 'a state \<Rightarrow> 'a state pmf"
+  where "step_1_lazy xs i state = do {
     let k = state_k state;
     let chi = state_chi state;
     insert_x_into_chi \<leftarrow> bernoulli_pmf (1/2^k);
@@ -25,8 +25,8 @@ definition lazy_step_1 :: "'a list \<Rightarrow> nat \<Rightarrow> 'a state \<Ri
 context with_threshold
 begin
 
-definition lazy_step_2 :: "'a list \<Rightarrow> nat \<Rightarrow> 'a state \<Rightarrow> 'a state pmf"
-  where "lazy_step_2 xs i state = do {
+definition step_2_lazy :: "'a list \<Rightarrow> nat \<Rightarrow> 'a state \<Rightarrow> 'a state pmf"
+  where "step_2_lazy xs i state = do {
     let k = state_k state;
     let chi = state_chi state;
 
@@ -40,7 +40,7 @@ definition lazy_step_2 :: "'a list \<Rightarrow> nat \<Rightarrow> 'a state \<Ri
   }"
 
 definition lazy_step :: "'a list \<Rightarrow> nat \<Rightarrow> 'a state \<Rightarrow> 'a state pmf"
-  where "lazy_step xs i state = lazy_step_1 xs i state \<bind> lazy_step_2 xs i"
+  where "lazy_step xs i state = step_1_lazy xs i state \<bind> step_2_lazy xs i"
 
 definition
   \<open>run_steps_from_state fold_fn step_fn state xs \<equiv>
@@ -52,7 +52,7 @@ definition lazy_algorithm :: "'a list \<Rightarrow> 'a state pmf"  where
 lemma lazy_step_cong:
   assumes "xs ! i = ys ! i"
   shows "lazy_step xs i = lazy_step ys i"
-  unfolding lazy_step_def lazy_step_1_def lazy_step_2_def
+  unfolding lazy_step_def step_1_lazy_def step_2_lazy_def
   using assms by (simp cong: if_cong)
 
 lemma lazy_algorithm_snoc:
@@ -78,13 +78,13 @@ next
 
   obtain \<omega>1 \<omega>2 where \<omega>:
     "\<omega>1 \<in> set_pmf (lazy_algorithm xs)"
-    "\<omega>2 \<in> set_pmf (lazy_step_1 (xs@[x]) ?n \<omega>1)"
-    "\<omega> \<in> set_pmf (lazy_step_2 (xs@[x]) ?n \<omega>2)"
+    "\<omega>2 \<in> set_pmf (step_1_lazy (xs@[x]) ?n \<omega>1)"
+    "\<omega> \<in> set_pmf (step_2_lazy (xs@[x]) ?n \<omega>2)"
     using snoc unfolding lazy_algorithm_snoc lazy_step_def by auto
 
   have "state_k \<omega>1 \<le> length xs" using snoc \<omega>(1) by simp
-  hence "state_k \<omega>2 \<le> length xs" using \<omega>(2) unfolding lazy_step_1_def by auto
-  hence "state_k \<omega> \<le> length xs + 1" using \<omega>(3) unfolding lazy_step_2_def
+  hence "state_k \<omega>2 \<le> length xs" using \<omega>(2) unfolding step_1_lazy_def by auto
+  hence "state_k \<omega> \<le> length xs + 1" using \<omega>(3) unfolding step_2_lazy_def
     by (cases "real (card (state_chi \<omega>2)) < threshold") (auto simp add:Let_def)
   thus ?case by simp
 qed
@@ -102,16 +102,16 @@ next
 
   obtain \<omega>1 \<omega>2 where \<omega>:
     "\<omega>1 \<in> set_pmf (lazy_algorithm xs)"
-    "\<omega>2 \<in> set_pmf (lazy_step_1 (xs@[x]) ?n \<omega>1)"
-    "\<omega> \<in> set_pmf (lazy_step_2 (xs@[x]) ?n \<omega>2)"
+    "\<omega>2 \<in> set_pmf (step_1_lazy (xs@[x]) ?n \<omega>1)"
+    "\<omega> \<in> set_pmf (step_2_lazy (xs@[x]) ?n \<omega>2)"
     using snoc unfolding lazy_algorithm_snoc lazy_step_def by auto
 
   have "state_chi \<omega>1 \<subseteq> set xs" using snoc \<omega>(1) by simp
   moreover have "state_chi \<omega>2 \<subseteq> insert x (state_chi \<omega>1)"
-    using \<omega>(2) unfolding lazy_step_1_def
+    using \<omega>(2) unfolding step_1_lazy_def
     by (auto simp add:nth_append cong:if_cong split:if_split_asm)
   ultimately have "state_chi \<omega>2 \<subseteq> set (xs@[x])" by auto
-  hence "state_chi \<omega> \<subseteq> set (xs@[x])" using \<omega>(3) unfolding lazy_step_2_def
+  hence "state_chi \<omega> \<subseteq> set (xs@[x])" using \<omega>(3) unfolding step_2_lazy_def
     by (cases "real (card (state_chi \<omega>2)) < threshold") (auto simp:Let_def)
   thus ?case by simp
 qed
@@ -176,7 +176,7 @@ proof -
         intro!: bind_pmf_cong map_pmf_cong
         simp flip: map_pmf_def
         simp add:
-          lazy_step_def lazy_step_1_def lazy_step_2_def
+          lazy_step_def step_1_lazy_def step_2_lazy_def
           step_1_no_fail_def step_2_no_fail_def
           map_bind_pmf bind_map_pmf map_pmf_comp Let_def)
 
